Test/dafny0/LiberalEquality.dfy
@@ -12,46 +12,94 @@ class Test<T> {
   predicate valid()
       reads this, a, b;
   {
-      a != null && b != null && a != b && a.Length == b.Length
+    a != null && b != null &&
+    a != b &&  // this is the kind of thing the liberal equalty rules are designed to support
+    a.Length == b.Length
   }
 }
 
-method m1<T, U>(t: T, u: U)
-   requires t != u; // Cannot compare type parameters (can only compare reference types that could be the same)
+method m0<T, U>(t: T, u: U, x: int)
+   requires t != u; // error: Cannot compare type parameters (can only compare reference types that could be the same)
+   requires u != x; // error: the liberal equality rules apply only if the top-level type is a reference type
 {
-   
 }
 
-method m2<T>(t: array<T>, a: array<int>)
-   requires t != null && a != null && t != a && t.Length == a.Length;
+method m1<T>(t: array<T>, a: array<int>, b: array3<T>, c: array3<int>)
+   requires t != null && a != null && b != null && c != null;
+   requires t != a && t.Length == a.Length;
+   requires b != c && b.Length0 == c.Length0 && b.Length1 == c.Length1 && b.Length2 == c.Length2;
+   requires t != b;  // error: these types are never the same
+   requires a != c;  // error: these types are never the same
+   requires t != c;  // error: these types are never the same
+   requires a != b;  // error: these types are never the same
 {
-
-}
-
-
-class Weird<T, U, V>
-{
-
-}
-
-
-method m3<T, V>(a: Weird<T, int, V>, b: Weird<T, bool, V>)
-   requires a == b; // Bad: second parameter can't be both bool and int.
-{
-
 }
 
 
-method m4<T, U, V>(a: Weird<T, U, V>, b: Weird<T, bool, V>)
+class Weird<T, U, V> { }
+
+method m2<T, V>(a: Weird<T, int, V>, b: Weird<T, bool, V>)
+   requires a == b; // error: second parameter can't be both bool and int.
+{
+}
+
+method m3<T, U, V>(a: Weird<T, U, V>, b: Weird<T, bool, V>)
   requires a == b;
 {
-
 }
 
+method m4<T>(a: Weird<T, T, bool>, b: Weird<T, bool, T>, c: Weird<T, int, T>)
+  requires b != c;  // error: this is like in m2 above
+  requires a != b;  // the types of a and b would be the same if T := bool
+  requires a != c;  // this is allowed by the liberal equality rules, which are simple minded;
+                    // but there isn't actually any way that the types of a and c could be the same
+{
+}
 
 // Just to make sure nothing went wrong.
 method m5(a: array<int>, b: array<bool>)
-   requires a == b; // Bad: never equal
+   requires a == b; // error: never equal
 {
+}
 
+iterator Iter<T>() { }
+
+method m6<T>(a: Iter<T>, b: Iter<int>)
+  requires a != b;
+{
+}
+
+method m7<T>(a: T -> int, b: int -> T, c: int -> int)
+  requires a != c;  // error: arrow types don't fall under the liberal equality rules
+  requires b != c;  // error: ditto
+{
+}
+
+type Syn<U> = Weird<U, U, int>
+
+method m8<T,U>(a: Weird<int,int,int>, b: Syn<int>, c: Weird<T, bool, U>, d: Syn<T>, e: Syn<bool>)
+  requires a != b;  // no prob -- the types are always equal
+  requires b != d;  // allowed
+  requires c != d;  // allowed
+  requires b != e;  // error: these can't be the same type, ever
+{
+}
+
+datatype List<X> = Nil | Cons(X, List<X>)
+type ListSynonym<X,Y> = List<Y>
+type Wrapper<T> = T
+
+method m9<T>(a: array<List<int>>, b: array<List<bool>>,
+             c: array<ListSynonym<T,int>>, d: array<ListSynonym<bool,int>>,
+             e: array<ListSynonym<int,T>>, f: array<ListSynonym<real,Wrapper<int>>>)
+  requires a != b;  // error
+  requires a != c;
+  requires b != c;  // error
+  requires c != d;
+  requires a != e;
+  requires b != e;
+  requires d != e;
+  requires a != f;
+  requires b != f;  // error
+{
 }
