Test/hofs/Consequence.dfy
@@ -1,9 +1,10 @@
 // RUN: %dafny /compile:0 "%s" > "%t"
 // RUN: %diff "%s.expect" "%t"
 
-method Check() {
-  var f : nat -> nat;
-  assume f.requires(0);
-  var i : nat := f(0);
-}
+newtype Nat = x | 0 <= x
 
+method Check() {
+  var f : Nat -> Nat;
+  assume f.requires(0);
+  var i : Nat := f(0);
+}
